Got the main lemma about the algorithm
Everything except the list has been proven

Monad_Play Around/DNFP/Dutch_National_Flag_Monad.thy
@@ -241,77 +241,6 @@ lemma dnfp_aux6: "spec (\<lambda>y. mset (xs e) = mset (xs y)) (dnfp_mon v) (\<l
   apply(simp add: spec_def)
   by (simp add: skip_def)
 
-lemma dnfp_aux7: "spec (\<lambda>y. i y \<le> high y \<and> high y - i y \<le> n) (dnfp_mon n) (\<lambda>x y. high y = i y)"
-  apply(induction n rule: dnfp_mon.induct)
-    apply(simp add: spec_def)    
-   apply (simp add: skip_def)    
-  apply(simp only: caseN)  
-  apply(intro get_rule; intro allI; clarify)
-  apply(intro cond_rule)
-  apply(simp add: loop_update_action_def)
-  apply(intro get_rule; intro allI; clarify)            
-  apply(intro seq_rule[of _ _ "(\<lambda>x y. i y \<le> high y \<and> high y - i y \<le> n)"])
-     apply(intro conj_rule_right)              
-
-    apply(intro cond_rule)
-  apply(simp add: inc_lowbound_def)        
-   apply(intro get_rule; intro allI; simp)             
-  apply(intro seq_rule[of _ _ "(\<lambda>x y. i y < high y)"])          
-       apply(simp add: spec_def put_def xs_Env_def swap_def put_state_def get_state_def)    
-       apply(intro allI; simp)                                    
-   apply(intro get_rule; intro allI)                             
-  apply(intro seq_rule[of _ _ "(\<lambda>x y. i y \<le> high y)"])     
-       apply(simp add: spec_def put_def i_Env_def put_state_def get_state_def)
-       apply(intro allI; simp)                    
-     apply(intro get_rule; intro allI)                     
-       apply(simp add: spec_def put_def low_Env_def put_state_def get_state_def)    
-                                 
-     apply(simp add: dec_highbound_def)                 
-  apply(intro get_rule; intro allI; simp)              
- apply(intro seq_rule[of _ _ "(\<lambda>x y. i y \<le> high y)"])        
-     apply(simp add: spec_def put_def high_Env_def put_state_def get_state_def)
-       apply linarith 
-         apply(intro allI; simp)            
-      apply(intro get_rule; intro allI; simp)                       
-     apply(simp add: spec_def put_def xs_Env_def put_state_def get_state_def)
-                                         
-     apply(simp add: inc_index_def)                
-      apply(intro get_rule; intro allI; simp)                       
-    apply(simp add: spec_def put_def i_Env_def put_state_def get_state_def)
-
-    apply(intro cond_rule)
-      apply(simp add: inc_lowbound_def)                  
-      apply(intro get_rule; intro allI; simp)       
-(*I need some help here*)                                      
- apply(intro seq_rule[of _ _ "(\<lambda>x y. high y - i y \<le> n \<and> high e = high y \<and> i e = i y)"])          
-      apply(simp add: spec_def put_def xs_Env_def swap_def put_state_def get_state_def)    
-  defer                               
-       apply(intro allI; simp)
-  apply(intro get_rule; intro allI)                             
- apply(intro seq_rule[of _ _ "(\<lambda>x y. high y - i y \<le> n)"])   
-      apply(simp add: spec_def put_def i_Env_def put_state_def get_state_def)
-  apply linarith                                    
-        apply(intro allI; simp)   
-    apply(intro get_rule; intro allI)
-      apply(simp add: spec_def put_def low_Env_def put_state_def get_state_def)    
-                                  
-      apply(simp add: dec_highbound_def)
-      apply(intro get_rule; intro allI; simp)          
-(*I need some help here*)
-  apply(intro seq_rule[of _ _ "(\<lambda>x y. high y - i y \<le> n)"])
-       apply(simp add: spec_def put_def high_Env_def put_state_def get_state_def)  
-
-       defer                        
-  defer
-      apply(simp add: inc_index_def)     
-  apply(intro get_rule; intro allI; simp) 
-       apply(simp add: spec_def put_def i_Env_def put_state_def get_state_def run_state_def)     
-  defer                                   
-      apply(intro allI; simp)    
-   apply(simp add: spec_def put_def i_Env_def put_state_def get_state_def run_state_def)
-  sorry
-
-
 subsection\<open>DNFP proof\<close>
 lemma dnfp_prepost: "spec (dnfp_pre n e) (dnfp_mon n) (GG (dnfp_post e))"
   apply(induction rule: dnfp_mon.induct)
@@ -320,7 +249,7 @@ lemma dnfp_prepost: "spec (dnfp_pre n e) (dnfp_mon n) (GG (dnfp_post e))"
    apply (simp add: skip_def)
   apply(intro conj_rule_right; simp only: caseN)
    apply(intro get_rule; intro allI; clarify)
-  apply(intro cond_rule)
+   apply(intro cond_rule; simp)
   apply(simp add: loop_update_action_def)
   apply(intro get_rule; intro allI; clarify)
   apply(intro seq_rule[of _ _ "(\<lambda>x y. length (xs e) = length (xs y))"])
@@ -507,20 +436,6 @@ lemma dnfp_prepost: "spec (dnfp_pre n e) (dnfp_mon n) (GG (dnfp_post e))"
   using dnfp_aux6 apply blast
   by(simp add: spec_def skip_def)
 
-(*
-  add precondition:
-  Everything outside n is sorted
-  high to n
-  And finally everything should be sorted
-  Post condition high = i 
-*)
-
-definition pre_dnfp_mon where
-"pre_dnfp_mon n e \<equiv> high e - i e = n
-                    \<and> dnfp_precondition e
-                    \<and> high e - i e = n
-                    \<and> invariants_Env e "
-
 subsection\<open>Invariants proof\<close>
 lemma dnfp_invariantRed: "spec (dnfp_inv1) (dnfp_mon n) (GG dnfp_inv1)"
   unfolding dnfp_inv1_def dnfp_pre_aux_def GG_def 
@@ -579,7 +494,7 @@ lemma dnfp_invariantBlue: "spec dnfp_inv3 (dnfp_mon n) (GG dnfp_inv3)"
      apply(simp add: spec_def)
   by(simp add: skip_def)
 
- text\<open>Main proof\<close>
+section\<open>Main proof\<close>
 definition dnfp_mon_inv :: "env \<Rightarrow> bool" where
 "dnfp_mon_inv e \<equiv> ((dnfp_inv3 e) \<and> (dnfp_inv2 e) \<and> (dnfp_inv1 e))"
 
@@ -591,18 +506,196 @@ definition dnfp_post_spec where
 
 lemma dnfp_mon_isSorted: "dnfp_post_spec e \<Longrightarrow> sorted (xs e)" 
   unfolding  dnfp_post_spec_def dnfp_mon_inv_def
-  sledgehammer
   by (smt Suc_1 Suc_leD dnfp_inv1_def dnfp_inv2_def dnfp_inv3_def high_invariant_is_2_Env_def invariant_low_to_j_is_1_Env_def less_numeral_extra(1) less_or_eq_imp_le less_trans low_invariant_is_0_Env_def not_less sorted_iff_nth_mono_less)
 
 definition dnfp_post_spec1 where
 "dnfp_post_spec1 e \<equiv> dnfp_mon_inv e \<and> i e = high e \<and> sorted(xs e)"
 
-lemma dnfp_mon_main: "spec (dnfp_mon_inv) (dnfp_mon n) (GG (dnfp_post_spec1))"
-  unfolding GG_def dnfp_post_spec1_def
-  apply(intro conj_rule_right)
-    apply (metis GG_def dnfp_mon_invariants strengthen_rule)
-   defer
+definition range_0:: "env \<Rightarrow> nat array" where
+"range_0 e \<equiv> nths (xs e) (set(upt 0 (low e)))"
+
+definition range_1:: "env \<Rightarrow> nat array" where
+"range_1 e \<equiv> nths (xs e) (set(upt (low e) (i e)))"
+
+definition range_2:: "env \<Rightarrow> nat array" where
+"range_2 e \<equiv> nths (xs e) (set(upt (high e) (length (xs e))))"
+
+lemma as: "nths x {0..<z} = take z x"
+  by (simp add: atLeast0LessThan)
+
+(*I don't get why I can't prove this*)
+lemma as1: "\<lbrakk>n = length x; z < n\<rbrakk> \<Longrightarrow> nths x {0..<z} @ nths x {z..<n}= take n x"
+  apply(induction n arbitrary: x)
+   apply simp
   sorry
 
+lemma complete_range_aux: "\<lbrakk>n = length x; z < length x\<rbrakk> \<Longrightarrow> nths x {0..<z} @ nths x {z..<n} = x"
+  apply(induction n arbitrary: z)
+   apply simp
+  by (simp add: as1)
+
+
+lemma complete_range: "\<lbrakk>z \<le> y; n = length x; y < length x\<rbrakk> \<Longrightarrow> nths x {0..<z} @ nths x {z..<y} @ nths x {y..<n} = x"
+  apply(induction n arbitrary: z y x)
+   apply simp
+  sorry
+
+lemma range_isComplete: "\<lbrakk>dnfp_precondition e; high e = i e\<rbrakk> \<Longrightarrow> concat[range_0 e, range_1 e,  range_2 e] = xs e"
+  unfolding range_0_def range_1_def range_2_def dnfp_precondition_def
+  apply(auto)
+  by (metis append.simps(1) append_Nil2 atLeastLessThan0 atLeastLessThan_empty_iff complete_range le0 le_SucE le_neq_implies_less le_numeral_extra(3) le_zero_eq length_0_conv less_Suc_eq_0_disj nths_empty same_append_eq set_upt zero_induct)
+
+definition sorted_range_get:: "env \<Rightarrow> nat array" where
+"sorted_range_get e \<equiv> range_0 e @ range_1 e @ range_2 e"
+
+definition sorted_range:: "env \<Rightarrow> bool" where
+"sorted_range e \<equiv> sorted(sorted_range_get e)"
+
+lemma range_0_isZero: "low_invariant_is_0_Env e \<Longrightarrow> \<forall>x \<in> set(range_0 e). x = 0"
+  unfolding low_invariant_is_0_Env_def range_0_def
+  by (smt atLeast_upt lessThan_iff mem_Collect_eq set_nths)
+
+lemma range_0_sorted: "dnfp_mon_inv e \<Longrightarrow> sorted (range_0 e)"
+  unfolding dnfp_mon_inv_def dnfp_inv3_def dnfp_inv2_def dnfp_inv1_def range_1_def dnfp_precondition_def
+  by (metis eq_iff less_trans nth_mem range_0_isZero sorted_iff_nth_mono_less)
+
+lemma range_1_isOne: "invariant_low_to_j_is_1_Env e \<Longrightarrow> \<forall>x \<in> set(range_1 e). x = 1"
+  unfolding invariant_low_to_j_is_1_Env_def range_1_def
+  by (smt atLeastLessThan_iff mem_Collect_eq set_nths set_upt)
+
+lemma range_1_sorted: "dnfp_mon_inv e \<Longrightarrow> sorted (range_1 e)"
+  by (smt diff_is_0_eq dnfp_inv2_def dnfp_mon_inv_def le_neq_implies_less length_take less_trans min.absorb2 nat_le_linear not_one_less_zero nth_mem range_1_def range_1_isOne sorted01 sorted_iff_nth_mono take_all)
+
+lemma ranges_sorted: "\<lbrakk>invariant_low_to_j_is_1_Env e; low_invariant_is_0_Env e\<rbrakk> \<Longrightarrow> sorted(range_0 e @ range_1 e)"
+  by (metis less_trans nat_le_linear not_one_le_zero nth_mem range_0_isZero range_1_isOne sorted_append sorted_iff_nth_mono_less)
+
+lemma range_2_isTwo: "high_invariant_is_2_Env e \<Longrightarrow> \<forall>x \<in> set(range_2 e). x = 2"
+  unfolding high_invariant_is_2_Env_def range_2_def
+  by (smt atLeastLessThan_iff mem_Collect_eq set_nths set_upt)
+
+lemma range_2_sorted: "dnfp_mon_inv e \<Longrightarrow> sorted (range_2 e)"
+  by (metis dnfp_inv3_def dnfp_mon_inv_def eq_iff less_trans nth_mem range_2_isTwo sorted_sorted_wrt sorted_wrt_iff_nth_less)
+
+lemma "dnfp_mon_inv e \<Longrightarrow> sorted(sorted_range_get e)"
+  by (metis Suc_1 dnfp_inv1_def dnfp_inv2_def dnfp_inv3_def dnfp_mon_inv_def lessI less_imp_le_nat range_0_isZero range_0_sorted range_1_isOne range_1_sorted range_2_isTwo range_2_sorted sorted_append sorted_range_get_def zero_le)
+
+lemma sorted_aux: "dnfp_mon_inv e \<Longrightarrow> sorted_range e"
+  unfolding sorted_range_def
+  by (metis Suc_1 dnfp_inv1_def dnfp_inv2_def dnfp_inv3_def dnfp_mon_inv_def lessI less_imp_le_nat range_0_isZero range_0_sorted range_1_isOne range_1_sorted range_2_isTwo range_2_sorted sorted_append sorted_range_get_def zero_le)
+
+lemma "sorted_range e \<and> i e = high e \<and> dnfp_precondition e \<Longrightarrow> sorted (xs e)"
+  unfolding sorted_range_def sorted_range_get_def dnfp_precondition_def
+  using dnfp_precondition_def range_isComplete by auto
+
+definition dnfp_mon_spec where
+"dnfp_mon_spec e \<equiv> dnfp_precondition e
+                    \<and> dnfp_mon_inv e
+                    \<and> sorted_range e"
+
+lemma dnfp_mon_main: "spec (dnfp_mon_spec) (dnfp_mon n) (GG dnfp_mon_spec)"
+  unfolding GG_def dnfp_mon_spec_def
+  apply(induction n rule: dnfp_mon.induct)
+    apply(simp add: spec_def)
+   apply(simp add: skip_def)
+  apply(simp only: caseN)
+  apply(intro get_rule; intro allI; clarify)
+  apply(intro cond_rule)
+   apply(simp add: loop_update_action_def)
+   apply(intro get_rule; intro allI; clarify)
+   apply(intro seq_rule[of _ _ "(\<lambda>x e. dnfp_precondition e \<and> dnfp_mon_inv e \<and> sorted_range e)"])
+    apply(intro cond_rule)
+      apply(intro conj_rule_right; simp)
+  apply (smt GG_def dnfp_inv1_def dnfp_mon_inv_def inc_lowbound_inv1_aux_def inc_lowbound_inv1_def inc_lowbound_invariantRed less_numeral_extra(1) loop_update_action_pre_def spec_def split_beta')
+  apply (smt GG_def Pair_inject dnfp_inv1_def dnfp_inv2_def dnfp_inv3_def dnfp_mon_inv_def inc_lowbound_inv1_aux_def inc_lowbound_inv1_def inc_lowbound_inv2_aux_def inc_lowbound_inv2_def inc_lowbound_inv3_aux_def inc_lowbound_inv3_def inc_lowbound_invariantBlue inc_lowbound_invariantRed inc_lowbound_invariantWhite less_one loop_update_action_pre_def spec_def split_beta')
+  apply (smt Dutch_National_Flag_Monad.sorted_aux GG_def dnfp_inv1_def dnfp_inv2_def dnfp_inv3_def dnfp_mon_inv_def inc_lowbound_inv1_aux_def inc_lowbound_inv1_def inc_lowbound_inv2_aux_def inc_lowbound_inv2_def inc_lowbound_inv3_aux_def inc_lowbound_inv3_def inc_lowbound_invariantBlue inc_lowbound_invariantRed inc_lowbound_invariantWhite less_numeral_extra(1) loop_update_action_pre_def spec_def split_beta')
+      apply(intro conj_rule_right)
+        apply (smt GG_def Pair_inject dec_highbound_inv1_aux_def dec_highbound_inv1_def dec_highbound_invariantRed dnfp_inv1_def dnfp_mon_inv_def loop_update_action_pre_def spec_def split_beta')
+      apply (smt GG_def Pair_inject dec_highbound_inv1_aux_def dec_highbound_inv1_def dec_highbound_inv2_aux_def dec_highbound_inv2_def dec_highbound_inv3_aux_def dec_highbound_inv3_def dec_highbound_invariantBlue dec_highbound_invariantRed dec_highbound_invariantWhite dnfp_inv1_def dnfp_inv2_def dnfp_inv3_def dnfp_mon_inv_def loop_update_action_pre_def spec_def split_beta')
+      apply (smt Dutch_National_Flag_Monad.sorted_aux GG_def Pair_inject dec_highbound_inv1_aux_def dec_highbound_inv1_def dec_highbound_inv2_aux_def dec_highbound_inv2_def dec_highbound_inv3_aux_def dec_highbound_inv3_def dec_highbound_invariantBlue dec_highbound_invariantRed dec_highbound_invariantWhite dnfp_inv1_def dnfp_inv2_def dnfp_inv3_def dnfp_mon_inv_def loop_update_action_pre_def spec_def split_beta')
+      apply(intro conj_rule_right)
+        apply (smt GG_def Pair_inject dnfp_inv1_def dnfp_mon_inv_def inc_index_inv1_aux_def inc_index_inv1_def inc_index_invariantRed less_one loop_update_action_pre_def spec_def split_beta')
+     apply (smt GG_def Pair_inject dnfp_inv1_def dnfp_inv2_def dnfp_inv3_def dnfp_mon_inv_def inc_index_inv1_aux_def inc_index_inv1_def inc_index_inv2_aux_def inc_index_inv2_def inc_index_inv3_aux_def inc_index_inv3_def inc_index_invariantBlue inc_index_invariantRed inc_index_invariantWhite less_one loop_update_action_pre_def spec_def split_beta')
+  apply (smt Dutch_National_Flag_Monad.sorted_aux GG_def Pair_inject dnfp_inv1_def dnfp_inv2_def dnfp_inv3_def dnfp_mon_inv_def inc_index_inv1_aux_def inc_index_inv1_def inc_index_inv2_aux_def inc_index_inv2_def inc_index_inv3_aux_def inc_index_inv3_def inc_index_invariantBlue inc_index_invariantRed inc_index_invariantWhite less_one loop_update_action_pre_def spec_def split_beta')
+  apply blast
+  by(simp add: spec_def skip_def)
+
+(*
+  add precondition:
+  Everything outside n is sorted
+  high to n
+  And finally everything should be sorted
+  Post condition high = i 
+*)
+
+
+definition i_high_equal::"nat \<Rightarrow> env \<Rightarrow> bool"  where
+ "i_high_equal n e \<equiv> high e = i e"
+
+definition dnfp_mon_pre::"nat \<Rightarrow> env \<Rightarrow> bool"  where
+"dnfp_mon_pre n e \<equiv> dnfp_precondition e \<and> n = high e - i e"
+
+lemma aux1: "(spec (\<lambda>e. dnfp_precondition e \<and> n = high e - i e) (dnfp_mon n)
+                (\<lambda>x e. high e = i e)) \<Longrightarrow>
+           spec
+            (\<lambda>xa. ((dnfp_precondition xa \<and> Suc n = high xa - i xa) \<and>
+                   (high x, i x) = (high xa, i xa)) \<and>
+                  i x < high x)
+            (loop_update_action \<bind> (\<lambda>_. dnfp_mon n)) (\<lambda>x e. high e = i e)"
+  apply(intro seq_rule[of _ _ "(\<lambda>x e. dnfp_precondition e
+                                \<and> n = high e - i e)"])
+   apply(simp add: loop_update_action_def)
+   apply(intro get_rule; intro allI; clarify)
+   apply(intro cond_rule)
+     apply(simp add: inc_lowbound_def)
+     apply(intro get_rule; intro allI; simp)
+  apply(intro seq_rule[of _ _ "(\<lambda>x e. Suc n = high e - i e \<and> high e > i e \<and> dnfp_precondition e)"])
+      apply(simp add: spec_def swap_def xs_Env_def put_def get_state_def put_state_def dnfp_precondition_def)
+   apply(intro allI; simp)
+      apply(intro get_rule; intro allI)
+  apply(intro seq_rule[of _ _ "(\<lambda>x e. n = high e - i e \<and> dnfp_precondition e \<and> i e > low e)"])
+  apply(simp add: spec_def i_Env_def put_def get_state_def put_state_def dnfp_precondition_def)
+  apply linarith
+   apply(intro allI; simp)
+      apply(intro get_rule; intro allI; simp)
+       apply(simp add: spec_def low_Env_def put_def get_state_def put_state_def dnfp_precondition_def)
+     apply(simp add: dec_highbound_def)
+     apply(intro get_rule; intro allI; simp)
+  apply(intro seq_rule[of _ _ "(\<lambda>x e. n = high e - i e \<and> dnfp_precondition e)"])
+     apply(simp add: spec_def high_Env_def put_def get_state_def put_state_def dnfp_precondition_def)
+  apply linarith
+   apply(intro allI; simp)
+      apply(intro get_rule; intro allI; simp)
+        apply(simp add: spec_def swap_def xs_Env_def put_def get_state_def put_state_def dnfp_precondition_def)
+        apply(simp add: inc_index_def)
+      apply(intro get_rule; intro allI; simp)
+   apply(simp add: spec_def i_Env_def put_def get_state_def put_state_def dnfp_precondition_def)
+  apply linarith
+  by blast
+
+lemma dnfp_mon_main_aux: "spec (dnfp_mon_pre n) (dnfp_mon n) (GG (i_high_equal n))"
+  unfolding GG_def dnfp_mon_pre_def dnfp_mon_spec_def i_high_equal_def
+  apply(induction n rule: dnfp_mon.induct)
+    apply(simp add: spec_def)
+   apply(simp add: skip_def)
+  apply (simp add: dnfp_precondition_def)
+  apply(simp only: caseN)
+   apply(intro get_rule; intro allI; clarify)
+  apply(intro cond_rule)
+  using aux1 apply blast
+  by(simp add: spec_def skip_def dnfp_precondition_def)
+
+definition dnfp_mon_spec_aux:: "nat \<Rightarrow> env \<Rightarrow> bool" where
+"dnfp_mon_spec_aux n e \<equiv> n = high e - i e \<and> dnfp_mon_spec e"
+
+definition list_sorted where
+"list_sorted e \<equiv> sorted(xs e)"
+
+lemma dnfp_mon_main_list_sorted: "spec (dnfp_mon_spec_aux n) (dnfp_mon n) (GG list_sorted)"
+  unfolding GG_def dnfp_mon_spec_aux_def  list_sorted_def
+  apply(induction n rule: dnfp_mon.induct)
+    apply(simp add: spec_def)
+   apply(simp add: skip_def)
+  apply (simp add: dnfp_mon_isSorted dnfp_mon_spec_def dnfp_post_spec_def dnfp_precondition_def)
+  by (smt GG_def dnfp_mon_invariants dnfp_mon_isSorted dnfp_mon_main_aux dnfp_mon_pre_def dnfp_mon_spec_def dnfp_post_spec_def i_high_equal_def spec_def split_beta')
 
 end
